\documentclass[12pt]{article}
\input{../preamble.tex}

\begin{document}
\centerline {\textsf{\textbf{\LARGE{Homework 1}}}}
\centerline {Jaden Wang}
\vspace{.15in}

\begin{problem}[1.1.1]
\begin{enumerate}[label=(\alph*)]
	\item 
	\begin{align*}
	u^* &= -Q^{-1}S \\
	    &= - \begin{pmatrix} -2&-1\\-1&-1 \end{pmatrix} \begin{pmatrix} 0\\1 \end{pmatrix}  \\
	    &= \begin{pmatrix} 1\\1 \end{pmatrix} 
\end{align*}
Since $ Q < 0$,  $ u^* $ is a global maximum. Then
\begin{align*}
	L^* &= -\frac{1}{2} S^{T}Q^{-1}S= \frac{1}{2} S^{T}u^* \\
	    &= \frac{1}{2} \begin{pmatrix} 0&1 \end{pmatrix} \begin{pmatrix} 1\\1 \end{pmatrix}  \\
	&= \frac{1}{2} 
\end{align*}
\begin{align*}
	L_u &= Qu + S \\
	&= \begin{pmatrix} -u_1+u_2\\u_1-2u_2 + 1 \end{pmatrix}  
\end{align*}
\item
\begin{align*}
	u^* &= - \frac{1}{3} \begin{pmatrix} 2&-1\\-1&-1 \end{pmatrix} \begin{pmatrix} 0\\1 \end{pmatrix} \\
	&= \begin{pmatrix} \frac{1}{3}\\\frac{1}{3} \end{pmatrix}  \\
\end{align*}
Since $ Q$ is indefinite,  $ u^* $ is a saddle point.
\begin{align*}
	L^* &= \frac{1}{2} S^{T} u^*  \\
	    &= \frac{1}{2} \begin{pmatrix} 0&1 \end{pmatrix} \begin{pmatrix} \frac{1}{3} \\ \frac{1}{3} \end{pmatrix}  \\
	    &= \frac{1}{6} 
\end{align*}

\begin{align*}
	L_u &= Qu + S \\
	&= \begin{pmatrix} -u_1+u_2\\u_1+2u_2+1 \end{pmatrix} 
\end{align*}
\end{enumerate}

TODO
\end{problem}
\begin{problem}[1.1.2]
We see that
\begin{align*}
Q= \begin{pmatrix} 2&-1\\-1&2 \end{pmatrix}, S= \begin{pmatrix} 3\\0 \end{pmatrix} 
\end{align*}
So
\begin{align*}
	x^* &= -Q^{-1}S = - \frac{1}{3} \begin{pmatrix} 2&1\\1&2 \end{pmatrix} \begin{pmatrix} 3\\0 \end{pmatrix}  \\
	&= \begin{pmatrix} -2\\-1 \end{pmatrix}   
\end{align*}
So 


\end{problem}

\begin{problem}[1.1.3]
\begin{align*}
	\nabla f(x,y) = \begin{pmatrix} 2x\\4y^3 \end{pmatrix} 
\end{align*}
So $ \nabla f(0,0) = 0$, indeed a critical point. The Hessian is
\begin{align*}
	\nabla ^2 f(x,y) = \begin{pmatrix} 2&0\\0&12y^2 \end{pmatrix} 
\end{align*}
which is positive semidefinite and thus singular at the origin. 

Since $ x^2 \geq 0$ and $ y^{4} \geq 0$, it is clear that $ f(x,y) \geq 0$. So  $ f(0,0)=0$ is indeed a minimum of  $ f$.
\end{problem}

\begin{problem}[1.2.1]
The cost function is $ L(x,y) = \frac{1}{2} (x-20)^2 + \frac{1}{2}(y-30)^2$ and the constraint is $ F(x,y)= y-\sqrt{3}x = 0$. The Hamiltonian is
\begin{align*}
	H(x,y) = L(x,y)+ \lambda F(x,y).
\end{align*}
Then
\begin{align*}
	H_x &= x-20 - \sqrt{3} \lambda =0\\
	H_y &= y-30 + \lambda = 0 \\
	H_\lambda &= y- \sqrt{3} x=0 
\end{align*}
Solving this yields $ x = \frac{1}{2}(15\sqrt{3}+10) $ and $ y = \frac{1}{2}(45+10\sqrt{3}) $. The distance is then $ d^* = \sqrt{x^2+y^2} =36 $ miles. Thus the time is about $ 36 / 10 = 3.6$ hours.
\end{problem}

\begin{problem}[1.2.2]
The cost function is $ L(x_3,y_3) = \frac{1}{2}(x_3-x_1)^2 + \frac{1}{2} (y_3-y_1)^2 + \frac{1}{2}(x_3-x_2)^2 + \frac{1}{2} (y_3-y_2)^2$. The constraint is $ F(x_3,y_3) = \frac{1}{2}(x_3-x_1)^2 + \frac{1}{2} (y_3-y_1)^2 - \frac{1}{2}(x_3-x_2)^2 - \frac{1}{2} (y_3-y_2)^2 =0$. Therefore,
\begin{align*}
	H_{x_3} &= x_3-x_1 + x_3-x_2 + \lambda(x_3-x_1) - \lambda (x_3-x_2)=0\\
	H_{y_3} &= y_3-y_1 + y_3-y_2 + \lambda(y_3-y_1) - \lambda (y_3-y_2) \\
	H_\lambda &= 0 
\end{align*}
Solving this yields $ x_3 = $
\end{problem}
\end{document}
