\documentclass[12pt]{article}
\input{../preamble.tex}

\begin{document}
\centerline {\textsf{\textbf{\LARGE{Homework 4}}}}
\centerline {Jaden Wang}
\vspace{.15in}
\begin{problem}[1]
\begin{enumerate}[label=(\alph*)]
The Hamiltonian of the problem is given by
\begin{align*}
	H(x_1,x_2,u,p_1,p_2) = \frac{1}{2} u ^2+ p_1x_2+p_2(u-x_2). 
\end{align*}
The adjoint equations are given by
\begin{align*}
	\dot{p_1} &= -H_{x_1} = 0 \\
	\dot{p_2} &= -H_{x_2} = p_2-p_1 .
\end{align*}
The first-order condition demands
\begin{align*}
	H_u = u+p_2 &= 0\\
	u&= -p_2 .
\end{align*}
Plugging this into the differential equations yield
\begin{align*}
	\dot{x_1} &= x_2 \\
	\dot{x_2} &= -x_2-p_2 .
\end{align*}
Together with the adjoint equations, we have 4 first-order equations and require 4 boundary conditions.
\item Since all initial and final times and states are fixed, we have 4 boundary conditions $ x_1(0)=x_2(0)=0$, $ x_1(3)=1$, and $ x_2(3)=2$. Mathematica yields
\begin{align*}
	u(t) &= \frac{6e^{3+t}+6e^{t}-e^{6}+4e^{3}-3}{e^{6}+4e^{3}-5}\\
	&=-0.6811 + 0.2642 e^{t}.
\end{align*}
~\begin{figure}[H]
	\centering
	\includegraphics[width=0.3\textwidth]{./figures/4.1.png}
	\includegraphics[width=0.3\textwidth]{./figures/4.2.png}
	\includegraphics[width=0.3\textwidth]{./figures/4.3.png}
\end{figure}
\item When $ x_2(3)$ is free, in its place we instead have the transversality condition $ p_2(3) = 0$. This yields the solution
\begin{align*}
	u(t) &= -\frac{2e^3(e^{t}-e^{3})}{3e^{6}+4e^3-1 }\\
	&= 0.6256 - 0.0311e^{t} \\
\end{align*}
~\begin{figure}[H]
	\centering
	\includegraphics[width=0.3\textwidth]{./figures/4.4.png}
	\includegraphics[width=0.3\textwidth]{./figures/4.5.png}
	\includegraphics[width=0.3\textwidth]{./figures/4.6.png}
\end{figure}

\item I would add a final penalty term $ \Phi$:
\begin{align*}
	\mathcal{ J} = \underbrace{ \frac{1}{2} \left( (x_1(3)-1)^2+(x_2(3)-2)^2 \right)  }_{\Phi(3) } + \frac{1}{2} \int_0^3 u^2 dt .
\end{align*}
Then instead of $ p_1(3)=p_2(3)=0$, we have
\begin{align*}
	p_1(3) &= \Phi_{x_1}(3) = x_1(3)-1 \\
	p_2(3) &= \Phi_{x_2}(3) = x_2(3)-2 
\end{align*}
Then new control is
\begin{align*}
	u(t) &= \frac{8e^{3+t}+6e^{t}+e^{6}+4e^3-3}{7e^{6}+8e^3-7}\\
	&= 0.1615+0.056 e^{t} .
\end{align*}
~\begin{figure}[H]
	\centering
	\includegraphics[width=0.3\textwidth]{./figures/4.7.png}
	\includegraphics[width=0.3\textwidth]{./figures/4.8.png}
	\includegraphics[width=0.3\textwidth]{./figures/4.9.png}
\end{figure}
We see that $ x_1(3) = 0.8385$ and $ x_2(3) = 0.7142$, which are not very close to $ (1,2)$. To improve accuracy, I would increase the weight of the penalty term. We see that the cost in part (a) is  $ 4.2859$. The cost as a function of the weight coefficient  $ c$ is shown in the figure below:
~\begin{figure}[H]
	\centering
	\includegraphics[width=0.4\textwidth]{./figures/4.10.png}
	\caption{We see that as the weight increases, the cost approaches that of the cost (orange) in part (a) asymptotically.}
\end{figure}
And we indeed see that the solution ends much closer to $ (1,2)$ when the weight is high:
~\begin{figure}[H]
	\centering
	\includegraphics[width=0.4\textwidth]{./figures/4.11.png}
	\caption{Blue is optimal path from part (a), green is part (c) with weight 100, and orange is part (c) with weight 1.}
\end{figure}

\item It is clear that $ \Psi = \begin{pmatrix} 2&5 \end{pmatrix} $. By transversality condition from Equation 5.234, we have the boundary conditions
\begin{align*}
	\begin{pmatrix} -p_1(3)\\-p_2(3) \end{pmatrix} &= \begin{pmatrix} 2\\5 \end{pmatrix} \lambda 
\end{align*}
Together with the initial conditions $ x_1(0)=x_2(0)=0$ and the terminal condition $ 2 x_1(3) + 5x_2(3) = 20$, we have 5 boundary conditions for 4 differential equations and an unknown $ \lambda$. This allows us to solve by Mathematica and obtain the optimal control:
\begin{align*}
	u(t)=-p_2(t)= 1.4341+0.1071 e^{t}
\end{align*}
~\begin{figure}[H]
	\centering
	\includegraphics[width=0.3\textwidth]{./figures/4.12.png}
	\includegraphics[width=0.3\textwidth]{./figures/4.13.png}
	\includegraphics[width=0.3\textwidth]{./figures/4.14.png}
	\caption{We see that the solution indeed ends at the constraint.}
\end{figure}

\item We have the same $\Psi $ but $ h(t) = 20 +\frac{t^2}{ 2}$ so $ \dot{h}(t_f) = t_f$. When $ t_f$ is also free, based on Equation 5.234 we have the transversality conditions
\begin{align*}
	\begin{pmatrix} H(t_f)\\ -p_1(t_f)\\-p_2(t_f) \end{pmatrix} &= \begin{pmatrix} -t_f\\ 2\\5 \end{pmatrix} \lambda 
\end{align*}
Note that by plugging in $ u=-p_2$, we have
\begin{align*}
	H &= -\frac{1}{2} p_2^2+(p_1-p_2)x_2\\
	H(t_f)&= -\frac{25}{2} \lambda + 3x_2(t_f) = -t_f 
\end{align*}
Together with two initial conditions and the terminal condition
\begin{align*}
	2x_1(t_f) +5x_2(t_f) = 20 + \frac{t_f^2}{ 2},
\end{align*}
we have a total of 6 boundary conditions to match the 4 differential equations and two unknowns $ \lambda$ and $ t_f$. Mathematica yields
\end{enumerate}
\end{problem}
\begin{problem}[2]
The Hamiltonian is
\begin{align*}
	H = \frac{1}{2} u^2 + p(ax+bu)
\end{align*}
The adjoint equation is
\begin{align*}
	\dot{p} = -H_x = ap \implies p(t) = C e^{at}.
\end{align*}
And the first-order condition is
\begin{align*}
	H_u = u+bp = 0 \implies u=-bp
\end{align*}
Thus
\begin{align*}
	\dot{x} = ax-b^2p = ax - b^2 C e^{at}, \quad x(0)=x_0,x(tf) = 0
\end{align*}
We have $ x(t) = b^2 C t e^{at} + A e^{at}$, $ x(0) = A = x_0$, and
\begin{align*}
	x(t_f) = b^2 C t_f e^{at_f} + x_0 e^{at_f} &= 0 \\
	C &= - \frac{x_0}{ b^2 t_f}
\end{align*}
Thus,
\begin{align*}
	u(t) = -bp = -b \cdot \left( - \frac{x_0}{b^2 t_f} \right) e^{at}  = \frac{x_0}{ b t_f} e^{at}
\end{align*}
\end{problem}
\begin{problem}[3]
With the mixed constraint $ \psi(x_0,x_f) = x_f - x_0 = 0$, we can turn $ x_0,x_f$ into free variables by adding a term with Lagrange multiplier. Let $ \Phi(x_0,x_f) = \phi(x_f) + \lambda \psi(x_0,x_f)= \frac{1}{2}(x(t_f)-1)^2 + \lambda(x_f - x_0)$. The Hamiltonian is
\begin{align*}
	H = \frac{1}{2} (x^2+u^2)+pu .
\end{align*}
The adjoint equation is
\begin{align*}
	\dot{p}= -H_x = x
\end{align*}
The first-order condition says
\begin{align*}
	H_u = u +p=0 \implies u = -p .
\end{align*}
Since both $x(0), x(2)$ is free, from Equation 5.234 we have the transversality condition
 \begin{align*}
	 (\Phi_{x_0}+p ^{T}(t_0)) \delta x_0 + (\Phi_{x_f}- p ^{T}(t_f)	\delta x_f = 0
\end{align*}
where $ \delta x_0$ and $ \delta x_f$ can take any value. This forces that
\begin{align*}
	\Phi_{x_0} + p ^{T}(t_0) &=0 \\
	\Phi_{x_f} - p ^{T}(t_f) &= 0 
\end{align*}
Thus for this problem, we have
\begin{align*}
	p(0) &= -\Phi_{x_0} = -(- \lambda ) = \lambda\\
	p(2) &= \Phi_{x_f} = x(2) -1 + \lambda  
\end{align*}

Thus we have two boundary conditions for two differential equations. Mathematica yields
\begin{align*}
	x(t) = \frac{\lambda \cos (2-t) + \cos t - \lambda \cost t + \lambda \sin (2-t)}{ \cos 2 - \sin 2 }.
\end{align*}
Solving $ x(0) = x(2)$, we obtain  $ \lambda = \frac{\cos(2)-1}{ 2 \cos 2 + \sin 2-2} \approx 0.7364$.
\begin{align*}
	u(t) &= -p(t) = \frac{\lambda (\cos(2-t)-\sin(2-t)-\sin t)+ \sin t}{\cos 2 - \sin 2 }\\
	&= 0.5556 (\cos(2-t)-\sin(2-t)) + 0.1989 \sin t
\end{align*}
The associated cost is $ 1.8506$.
\end{problem}

\begin{problem}[4]
\begin{enumerate}[label=(\alph*)]
\item Since the cost $ \mathcal{ J} = t_f$, we have $ \Phi(t) = t$ and the Hamiltonian is
	\begin{align*}
		H= p_1(t) \cos \theta (t) + p_2(t) \sin \theta(t) + p_3(t) u(t) + p_4(t) v(t)
	\end{align*}
\item The adjoint equations are
\begin{align*}
	\begin{pmatrix} \dot{p_1}\\\dot{p_2}\\\dot{p_3}\\ \dot{p_4} \end{pmatrix} = \begin{pmatrix} -H_u\\-H_v\\-H_x\\-H_y \end{pmatrix} = \begin{pmatrix} p_3\\p_4\\0\\0 \end{pmatrix} 
\end{align*}
\item Since $ t_f, u(t_f),v(t_f)$ are free, by Equation 5.234 we have  the transversality conditions
	\begin{align*}
		H(t_f) + \Phi_t(t_f) = 0 \implies H(t_f) = -1 \\
		p_1(t_f) = \Phi_u = 0\\
		p_2(t_f) = \Phi_v = 0 .
	\end{align*}
\item Notice that $ p_3,p_4$ are constants, so $ p_1(t) = p_3t$ and $ p_2(t) = p_4t$ by the zero boundary conditions. First-order condition yields
\begin{align*}
	H_\theta = -p_1 \sin \theta(t) + p_2 \cos \theta(t) &= 0 \\
	\tan \theta^*(t)  &= \frac{p_2(t)}{ p_1(t)} = \frac{p_4}{ p_3}
\end{align*}
which is a constant! So are $ \cos \theta^* $ and $ \sin \theta^* $. Thus by the initial conditions $u(0)= \cos \gamma_0, v(0) = \sin \gamma_0$, we have $ u(t) = \cos \theta^* t$ and $ v(t) = \sin \theta^* $. By the initial conditions $x(0)=y(0)=0$, we have $ x(t) = \frac{1}{2} \cos \theta^* t^2 + \cos \gamma_0 t$ and $ y(t) = \frac{1}{2} \sin \theta^* t^2+ \sin \gamma_0 t$. By the terminal condition $ x(t_f)=x_f$ and  $ y(t_f)=0$, we have 
\begin{align*}
	x_f -\cos \gamma_0 t_f &= \frac{1}{2} \cos \theta^* t_f^2\\
	- \sin \gamma_0 t_f &= \frac{1}{2} \sin \theta^* t_f^2 
\end{align*}
Squaring both sides and adding the two equations together, we obtain the equation as desired:
\begin{align*}
	x_f^2-2\cos \gamma_0 t_f + (\cos \gamma_0^2+\sin \gamma_0^2) t_f^2 &= \frac{1}{4} (\cos^2\theta^* +\sin^2\theta^* )t_f^{4}\\
	4x_f^2-8 \cos \gamma_0 t_f + 4t_f^2 - t_f^{4} &= 0 
\end{align*}
So $ t_f$ must be the minimum positive solution of this equation.
\item By the above equation,
\begin{align*}
	\cos \theta^* &= 2\left(\frac{x_f}{t_f^2}+\frac{\cos \gamma_0}{ t_f}\right) \\
	\theta^* &= \arccos \left( 2\left(\frac{x_f}{t_f^2}+\frac{\cos \gamma_0}{ t_f^}\right)  \right)  
\end{align*}
\end{enumerate}
\end{problem}
\begin{problem}[5]
The cost has the Meyer form $ J = t_f$ so  $ \Phi(t) = t$. The Hamiltonian is
\begin{align*}
	H(x,y,p_1,p_2) &= p_1 r \cos \beta + p_2 r \sin \beta .
\end{align*}
The adjoint equations are
\begin{align*}
	\dot{p_1} &= -H_x = - p_1 \frac{x}{r} \cos \beta - p_2 \frac{x}{r} \sin \beta \\
	\dot{p_2} &= -H_y = p_1 \frac{y}{r} \cos \beta - p_2 \frac{x}{r} \sin \beta 
\end{align*}
Note that $ \dot{p_2} = \frac{y}{x} \dot{p_1}$. First-order condition yields
\begin{align*}
	H_{\beta} = -p_1 r \sin \beta + p_2 r \cos \beta &= 0 \\
	\tan \beta &= \frac{p_2}{p_1} 
\end{align*}
Thus we obtain $ p_2 = \tan \beta p_1$. Moreover, we see that
\begin{align*}
	p_2 \cos \beta - p_1 \sin \beta &= \frac{p_2p_1 - p_1 p_2}{ \sqrt{p_1^2+p_2^2} } \\
	&= 0 .
\end{align*}
Now we compute
\begin{align*}
	0=\frac{d}{dt} H_{ \beta} &= \dot{r} (-p_1 \sin \beta + p_2 \cos \beta) + r\left( -\frac{d}{dt}(p_1 \sin \beta) + \frac{d}{dt}(p_2 \cos \beta) \right)  \\
				0&=0 + r \left( -\dot{p_1} \sin \beta - p1 \cos \beta \dot{\beta} + \dot{p_2} \cos \beta - p_2 \sin \beta \dot{\beta} \right)   \\
				0&= -\dot{p_1} \sin \beta - p1 \cos \beta \dot{\beta} + \frac{y}{x} \dot{p_1} \cos \beta - p_1\tan \beta \sin \beta \dot{\beta} \\
				p_1 (cos \beta + \tan \beta \sin \beta) \dot{ \beta} &= \dot{p_1} \left( - \sin \beta + \frac{y}{x} \cos \beta \right)  \\
				p_1 (cos \beta + \tan \beta \sin \beta) \dot{ \beta} &= \left( p_1 \frac{x}{r} \cos \beta + \tan \beta p_1 \frac{x}{r} \sin \beta \right)  \left( \sin \beta - \frac{y}{x} \cos \beta \right)  \\
				\dot{\beta}&= \frac{x}{r} \left( \sin \beta - \frac{y}{x} \cos \beta \right)  \\
				\dot{\beta} &=  \frac{x}{r} sin \beta - \frac{y}{r} \cos \beta
\end{align*}
\end{problem}
\end{document}
